NoveltyTheory/All.lean
@@ -13,6 +13,7 @@ import NoveltyTheory.Models.SignatureTower
 import NoveltyTheory.Models.InvariantTower
 import NoveltyTheory.Models.BoundedRegimeDiagonal
 import NoveltyTheory.Models.ReducerDiagonal
+import NoveltyTheory.Models.DupRegimeTower
 import NoveltyTheory.Models.CausalExplanatoryOrders
 import NoveltyTheory.Models.GenCertPhase
 import NoveltyTheory.Models.SimulationVersusExplanation
